AncestorContexts 구현중 - ancestor_list 에 대한 'decreaser' 도 구현중!

src/study/Nemonuri.Study.CSharpSyntaxRewriter2.Modifier2/Nemonuri.StratifiedNodes.Indexes.fst
@@ -32,36 +32,6 @@ let get_indexes #t (ancestors:C.ancestor_list t)
   let hd::tl = ancestors in
   get_indexes_core hd tl
 
-(*
-private let rec are_indexes_of_core #t
-  (indexes:list nat)
-  (ancestors_hd:N.node t) (ancestors_tl:C.next_head_given_ancestor_list ancestors_hd)
-  : Pure bool 
-    (requires (L.length indexes) = (L.length ancestors_tl))
-    (ensures fun _ -> true)
-    (decreases indexes)
-  =
-  match ancestors_tl with
-  | [] -> true
-  | a_hd2::a_tl2 -> (
-      assert (C.is_parent a_hd2 ancestors_hd);
-      let i_hd::i_tl = indexes in
-      match ((C.get_child_index a_hd2 ancestors_hd) = i_hd) with
-      | false -> false
-      | true -> (are_indexes_of_core i_tl a_hd2 a_tl2)
-    )
-
-let are_indexes_of #t 
-  (indexes:list nat) (ancestors:C.ancestor_list t) 
-  : Pure bool
-    (requires (L.length indexes) = ((L.length ancestors) - 1))
-    (ensures fun _ -> true)
-    (decreases indexes)
-  =
-  let a_hd::a_tl = ancestors in
-  are_indexes_of_core indexes a_hd a_tl
-*)
-
 private let rec can_get_descendant_or_self_from_indexes_core #t
   (hd:N.node t) (reversed_indexes:list nat)
   : Tot bool (decreases reversed_indexes) =
@@ -103,5 +73,58 @@ let get_descendant_or_self_from_indexes #t
     (ensures fun _ -> true)
   =
   get_descendant_or_self_from_indexes_core hd (L.rev indexes)
+
+(*
+private let rec are_indexes_of_core #t
+  (indexes:list nat)
+  (ancestors_hd:N.node t) (ancestors_tl:C.next_head_given_ancestor_list ancestors_hd)
+  : Pure bool 
+    (requires (L.length indexes) = (L.length ancestors_tl))
+    (ensures fun _ -> true)
+    (decreases indexes)
+  =
+  match ancestors_tl with
+  | [] -> true
+  | a_hd2::a_tl2 -> (
+      assert (C.is_parent a_hd2 ancestors_hd);
+      let i_hd::i_tl = indexes in
+      match (i_hd < (N.get_children_length ancestors_hd)) && ((N.get_child_at ancestors_hd i_hd) = a_hd2) with
+      | false -> false
+      | true -> (are_indexes_of_core i_tl a_hd2 a_tl2)
+    )
+
+let are_indexes_of2 #t 
+  (indexes:list nat) (ancestors:C.ancestor_list t) 
+  : Pure bool
+    (requires (L.length indexes) = ((L.length ancestors) - 1))
+    (ensures fun _ -> true)
+    (decreases indexes)
+  =
+  let a_hd::a_tl = ancestors in
+  are_indexes_of_core indexes a_hd a_tl
+*)
+
+let has_index #t
+  (parent:N.node t) (child:N.node t) (index:nat)
+  : Pure bool 
+    (requires C.is_parent parent child)
+    (ensures fun _ -> true)
+  =
+  if not (index < (N.get_children_length parent)) then false else
+  ((N.get_child_at parent index) = child)
+
+
+let rec have_indexes #t
+  (ancestors:C.ancestor_list t) (indexes:list nat) 
+  : Tot bool 
+    (decreases indexes)
+  =
+  if not ((L.length indexes) = ((L.length ancestors) - 1)) then false else
+  if Nil? indexes then true else
+  let (i_hd::i_tl, a_hd::a_tl) = (indexes, ancestors) in
+  let a_hd2::a_tl2 = a_tl in
+  assert (C.is_parent a_hd2 a_hd);
+  if not (has_index a_hd2 a_hd i_hd) then false else
+  have_indexes a_tl i_tl
 
 //---|
