src/study/Nemonuri.Study.CSharpSyntaxRewriter2.Modifier2/Nemonuri.StratifiedNodes.AncestorContexts.Types.fst
@@ -1,0 +1,17 @@
+module Nemonuri.StratifiedNodes.AncestorContexts.Types
+
+module L = FStar.List.Tot
+module N = Nemonuri.StratifiedNodes.Nodes
+module C = Nemonuri.StratifiedNodes.Children
+module Common = Nemonuri.StratifiedNodes.Common
+module Id = Nemonuri.StratifiedNodes.Indexes
+
+//--- type definition ---
+
+type ancestor_context (t:eqtype) = 
+| AContext :
+  (ancestors: C.ancestor_list t) ->
+  (indexes:list nat{Id.have_indexes ancestors indexes}) ->
+  ancestor_context t
+
+//---|
