src/study/Nemonuri.Study.CSharpSyntaxRewriter2.Modifier2/Nemonuri.StratifiedNodes.AncestorContexts.fst
@@ -1,0 +1,71 @@
+module Nemonuri.StratifiedNodes.AncestorContexts
+
+module L = FStar.List.Tot
+module N = Nemonuri.StratifiedNodes.Nodes
+module C = Nemonuri.StratifiedNodes.Children
+module Common = Nemonuri.StratifiedNodes.Common
+module Id = Nemonuri.StratifiedNodes.Indexes
+module T = Nemonuri.StratifiedNodes.AncestorContexts.Types
+
+
+//--- members ---
+
+let get_ancestors #t
+  (ancestor_context:T.ancestor_context t)
+  : Tot (C.ancestor_list t)
+  =
+  T.AContext?.ancestors ancestor_context
+
+let get_indexes #t
+  (ancestor_context:T.ancestor_context t)
+  : Tot (list nat)
+  =
+  T.AContext?.indexes ancestor_context
+
+let is_prependable_to_ancestor_context #t
+  (node:N.node t) (index:nat) (ancestor_context:T.ancestor_context t)
+  : Tot bool
+  =
+  let ancestors = (get_ancestors ancestor_context) in
+  (C.is_concatenatable_to_ancestor_list node ancestors) &&
+  (Id.has_index (L.hd ancestors) node index)
+
+let prepend_to_ancestor_context #t
+  (node:N.node t) (index:nat) (ancestor_context:T.ancestor_context t)
+  : Pure (T.ancestor_context t)
+    (requires is_prependable_to_ancestor_context node index ancestor_context)
+    (ensures fun r -> 
+      ((L.tl (get_ancestors r)) = (get_ancestors ancestor_context)) &&
+      ((L.tl (get_indexes r)) = (get_indexes ancestor_context))
+    )
+  = 
+  let new_ancestors = C.concatenate_as_ancestor_list node (get_ancestors ancestor_context) in
+  let new_indexes = index::(get_indexes ancestor_context) in
+  T.AContext new_ancestors new_indexes
+
+let next_heads_given_ancestor_context #t (node:N.node t) (index:nat) =
+  ac:T.ancestor_context t{ is_prependable_to_ancestor_context node index ac }
+
+let heads_given_ancestor_context #t (node:N.node t) (index:nat) =
+  ac:T.ancestor_context t{
+    match (get_ancestors ac, get_indexes ac) with
+    | (_, []) -> false
+    | (a_hd::a_tl, i_hd::i_tl) ->
+      (a_hd = node) && (i_hd = index)
+  }
+
+let ancestor_context_given_selector (t:eqtype) (t2:Type) =
+  (node:N.node t) -> 
+  (index:nat) ->
+  (ancestors:next_heads_given_ancestor_context node index) ->
+  Tot t2
+
+//---|
+
+//--- proof ---
+
+
+
+//---|
+
+include Nemonuri.StratifiedNodes.AncestorContexts.Types
